# Brick element for linear 3d elasticity 

## Nomenclature 

### Coordinates of the current point 

``` 
[x , x , x ] 
  1   2   3
``` 

### Dimensions of the element 

``` 
[h , h , h ] 
  1   2   3
``` 

### Numbering of nodes 

``` 
node[1,1,1] = [x[1] = 0,x[2] = 0,x[3] = 0] 

node[1,1,2] = [x[1] = 0,x[2] = 0,x[3] = h[3]] 

node[1,2,1] = [x[1] = 0,x[2] = h[2],x[3] = 0] 

node[1,2,2] = [x[1] = 0,x[2] = h[2],x[3] = h[3]] 

node[2,1,1] = [x[1] = h[1],x[2] = 0,x[3] = 0] 

node[2,1,2] = [x[1] = h[1],x[2] = 0,x[3] = h[3]] 

node[2,2,1] = [x[1] = h[1],x[2] = h[2],x[3] = 0] 

node[2,2,2] = [x[1] = h[1],x[2] = h[2],x[3] = h[3]] 

``` 

## Shape functions and interpolation of the displacements 

``` 
N[1,1,1] = (1-x[1]/h[1])*(1-x[2]/h[2])*(1-x[3]/h[3]) 

N[1,1,2] = ((1-x[1]/h[1])*(1-x[2]/h[2])*x[3])/h[3] 

N[1,2,1] = ((1-x[1]/h[1])*x[2]*(1-x[3]/h[3]))/h[2] 

N[1,2,2] = ((1-x[1]/h[1])*x[2]*x[3])/(h[2]*h[3]) 

N[2,1,1] = (x[1]*(1-x[2]/h[2])*(1-x[3]/h[3]))/h[1] 

N[2,1,2] = (x[1]*(1-x[2]/h[2])*x[3])/(h[1]*h[3]) 

N[2,2,1] = (x[1]*x[2]*(1-x[3]/h[3]))/(h[1]*h[2]) 

N[2,2,2] = (x[1]*x[2]*x[3])/(h[1]*h[2]*h[3]) 

``` 

Testing numbering of vertices... 
OK 

Testing that interpolated displacements are correct at vertices... 
OK 

We get the following expressions for the displacements 

``` 
u[1] = xi[1]*u[1,[2,2,2]]*xi[2]*xi[3]+(1-xi[1])*u[1,[1,2,2]]*xi[2]*xi[3]+xi[1]*u[1,[2,1,2]]*(1-xi[2])*xi[3]+(1-xi[1])*u[1,[1,1,2]]*(1-xi[2])*xi[3]+xi[1]*u[1,[2,2,1]]*xi[2]*(1-xi[3])+(1-xi[1])*u[1,[1,2,1]]*xi[2]*(1-xi[3])+xi[1]*u[1,[2,1,1]]*(1-xi[2])*(1-xi[3])+(1-xi[1])*u[1,[1,1,1]]*(1-xi[2])*(1-xi[3]) 

u[2] = xi[1]*xi[2]*u[2,[2,2,2]]*xi[3]+xi[1]*(1-xi[2])*u[2,[2,1,2]]*xi[3]+(1-xi[1])*xi[2]*u[2,[1,2,2]]*xi[3]+(1-xi[1])*(1-xi[2])*u[2,[1,1,2]]*xi[3]+xi[1]*xi[2]*u[2,[2,2,1]]*(1-xi[3])+xi[1]*(1-xi[2])*u[2,[2,1,1]]*(1-xi[3])+(1-xi[1])*xi[2]*u[2,[1,2,1]]*(1-xi[3])+(1-xi[1])*(1-xi[2])*u[2,[1,1,1]]*(1-xi[3]) 

u[3] = xi[1]*xi[2]*xi[3]*u[3,[2,2,2]]+xi[1]*xi[2]*(1-xi[3])*u[3,[2,2,1]]+xi[1]*(1-xi[2])*xi[3]*u[3,[2,1,2]]+xi[1]*(1-xi[2])*(1-xi[3])*u[3,[2,1,1]]+(1-xi[1])*xi[2]*xi[3]*u[3,[1,2,2]]+(1-xi[1])*xi[2]*(1-xi[3])*u[3,[1,2,1]]+(1-xi[1])*(1-xi[2])*xi[3]*u[3,[1,1,2]]+(1-xi[1])*(1-xi[2])*(1-xi[3])*u[3,[1,1,1]] 

``` 

## Interpolation of the strains 

``` 
B[1,1,1,1,1,1] = -1/(4*h[1]) 
B[1,1,1,1,1,2] = -1/(4*h[1]) 
B[1,1,1,1,2,1] = -1/(4*h[1]) 
B[1,1,1,1,2,2] = -1/(4*h[1]) 
B[1,1,1,2,1,1] = 1/(4*h[1]) 
B[1,1,1,2,1,2] = 1/(4*h[1]) 
B[1,1,1,2,2,1] = 1/(4*h[1]) 
B[1,1,1,2,2,2] = 1/(4*h[1]) 
B[1,1,2,1,1,1] = 0 
B[1,1,2,1,1,2] = 0 
B[1,1,2,1,2,1] = 0 
B[1,1,2,1,2,2] = 0 
B[1,1,2,2,1,1] = 0 
B[1,1,2,2,1,2] = 0 
B[1,1,2,2,2,1] = 0 
B[1,1,2,2,2,2] = 0 
B[1,1,3,1,1,1] = 0 
B[1,1,3,1,1,2] = 0 
B[1,1,3,1,2,1] = 0 
B[1,1,3,1,2,2] = 0 
B[1,1,3,2,1,1] = 0 
B[1,1,3,2,1,2] = 0 
B[1,1,3,2,2,1] = 0 
B[1,1,3,2,2,2] = 0 
B[1,2,1,1,1,1] = -1/(8*h[2]) 
B[1,2,1,1,1,2] = -1/(8*h[2]) 
B[1,2,1,1,2,1] = 1/(8*h[2]) 
B[1,2,1,1,2,2] = 1/(8*h[2]) 
B[1,2,1,2,1,1] = -1/(8*h[2]) 
B[1,2,1,2,1,2] = -1/(8*h[2]) 
B[1,2,1,2,2,1] = 1/(8*h[2]) 
B[1,2,1,2,2,2] = 1/(8*h[2]) 
B[1,2,2,1,1,1] = -1/(8*h[1]) 
B[1,2,2,1,1,2] = -1/(8*h[1]) 
B[1,2,2,1,2,1] = -1/(8*h[1]) 
B[1,2,2,1,2,2] = -1/(8*h[1]) 
B[1,2,2,2,1,1] = 1/(8*h[1]) 
B[1,2,2,2,1,2] = 1/(8*h[1]) 
B[1,2,2,2,2,1] = 1/(8*h[1]) 
B[1,2,2,2,2,2] = 1/(8*h[1]) 
B[1,2,3,1,1,1] = 0 
B[1,2,3,1,1,2] = 0 
B[1,2,3,1,2,1] = 0 
B[1,2,3,1,2,2] = 0 
B[1,2,3,2,1,1] = 0 
B[1,2,3,2,1,2] = 0 
B[1,2,3,2,2,1] = 0 
B[1,2,3,2,2,2] = 0 
B[1,3,1,1,1,1] = -1/(8*h[3]) 
B[1,3,1,1,1,2] = 1/(8*h[3]) 
B[1,3,1,1,2,1] = -1/(8*h[3]) 
B[1,3,1,1,2,2] = 1/(8*h[3]) 
B[1,3,1,2,1,1] = -1/(8*h[3]) 
B[1,3,1,2,1,2] = 1/(8*h[3]) 
B[1,3,1,2,2,1] = -1/(8*h[3]) 
B[1,3,1,2,2,2] = 1/(8*h[3]) 
B[1,3,2,1,1,1] = 0 
B[1,3,2,1,1,2] = 0 
B[1,3,2,1,2,1] = 0 
B[1,3,2,1,2,2] = 0 
B[1,3,2,2,1,1] = 0 
B[1,3,2,2,1,2] = 0 
B[1,3,2,2,2,1] = 0 
B[1,3,2,2,2,2] = 0 
B[1,3,3,1,1,1] = -1/(8*h[1]) 
B[1,3,3,1,1,2] = -1/(8*h[1]) 
B[1,3,3,1,2,1] = -1/(8*h[1]) 
B[1,3,3,1,2,2] = -1/(8*h[1]) 
B[1,3,3,2,1,1] = 1/(8*h[1]) 
B[1,3,3,2,1,2] = 1/(8*h[1]) 
B[1,3,3,2,2,1] = 1/(8*h[1]) 
B[1,3,3,2,2,2] = 1/(8*h[1]) 
B[2,1,1,1,1,1] = -1/(8*h[2]) 
B[2,1,1,1,1,2] = -1/(8*h[2]) 
B[2,1,1,1,2,1] = 1/(8*h[2]) 
B[2,1,1,1,2,2] = 1/(8*h[2]) 
B[2,1,1,2,1,1] = -1/(8*h[2]) 
B[2,1,1,2,1,2] = -1/(8*h[2]) 
B[2,1,1,2,2,1] = 1/(8*h[2]) 
B[2,1,1,2,2,2] = 1/(8*h[2]) 
B[2,1,2,1,1,1] = -1/(8*h[1]) 
B[2,1,2,1,1,2] = -1/(8*h[1]) 
B[2,1,2,1,2,1] = -1/(8*h[1]) 
B[2,1,2,1,2,2] = -1/(8*h[1]) 
B[2,1,2,2,1,1] = 1/(8*h[1]) 
B[2,1,2,2,1,2] = 1/(8*h[1]) 
B[2,1,2,2,2,1] = 1/(8*h[1]) 
B[2,1,2,2,2,2] = 1/(8*h[1]) 
B[2,1,3,1,1,1] = 0 
B[2,1,3,1,1,2] = 0 
B[2,1,3,1,2,1] = 0 
B[2,1,3,1,2,2] = 0 
B[2,1,3,2,1,1] = 0 
B[2,1,3,2,1,2] = 0 
B[2,1,3,2,2,1] = 0 
B[2,1,3,2,2,2] = 0 
B[2,2,1,1,1,1] = 0 
B[2,2,1,1,1,2] = 0 
B[2,2,1,1,2,1] = 0 
B[2,2,1,1,2,2] = 0 
B[2,2,1,2,1,1] = 0 
B[2,2,1,2,1,2] = 0 
B[2,2,1,2,2,1] = 0 
B[2,2,1,2,2,2] = 0 
B[2,2,2,1,1,1] = -1/(4*h[2]) 
B[2,2,2,1,1,2] = -1/(4*h[2]) 
B[2,2,2,1,2,1] = 1/(4*h[2]) 
B[2,2,2,1,2,2] = 1/(4*h[2]) 
B[2,2,2,2,1,1] = -1/(4*h[2]) 
B[2,2,2,2,1,2] = -1/(4*h[2]) 
B[2,2,2,2,2,1] = 1/(4*h[2]) 
B[2,2,2,2,2,2] = 1/(4*h[2]) 
B[2,2,3,1,1,1] = 0 
B[2,2,3,1,1,2] = 0 
B[2,2,3,1,2,1] = 0 
B[2,2,3,1,2,2] = 0 
B[2,2,3,2,1,1] = 0 
B[2,2,3,2,1,2] = 0 
B[2,2,3,2,2,1] = 0 
B[2,2,3,2,2,2] = 0 
B[2,3,1,1,1,1] = 0 
B[2,3,1,1,1,2] = 0 
B[2,3,1,1,2,1] = 0 
B[2,3,1,1,2,2] = 0 
B[2,3,1,2,1,1] = 0 
B[2,3,1,2,1,2] = 0 
B[2,3,1,2,2,1] = 0 
B[2,3,1,2,2,2] = 0 
B[2,3,2,1,1,1] = -1/(8*h[3]) 
B[2,3,2,1,1,2] = 1/(8*h[3]) 
B[2,3,2,1,2,1] = -1/(8*h[3]) 
B[2,3,2,1,2,2] = 1/(8*h[3]) 
B[2,3,2,2,1,1] = -1/(8*h[3]) 
B[2,3,2,2,1,2] = 1/(8*h[3]) 
B[2,3,2,2,2,1] = -1/(8*h[3]) 
B[2,3,2,2,2,2] = 1/(8*h[3]) 
B[2,3,3,1,1,1] = -1/(8*h[2]) 
B[2,3,3,1,1,2] = -1/(8*h[2]) 
B[2,3,3,1,2,1] = 1/(8*h[2]) 
B[2,3,3,1,2,2] = 1/(8*h[2]) 
B[2,3,3,2,1,1] = -1/(8*h[2]) 
B[2,3,3,2,1,2] = -1/(8*h[2]) 
B[2,3,3,2,2,1] = 1/(8*h[2]) 
B[2,3,3,2,2,2] = 1/(8*h[2]) 
B[3,1,1,1,1,1] = -1/(8*h[3]) 
B[3,1,1,1,1,2] = 1/(8*h[3]) 
B[3,1,1,1,2,1] = -1/(8*h[3]) 
B[3,1,1,1,2,2] = 1/(8*h[3]) 
B[3,1,1,2,1,1] = -1/(8*h[3]) 
B[3,1,1,2,1,2] = 1/(8*h[3]) 
B[3,1,1,2,2,1] = -1/(8*h[3]) 
B[3,1,1,2,2,2] = 1/(8*h[3]) 
B[3,1,2,1,1,1] = 0 
B[3,1,2,1,1,2] = 0 
B[3,1,2,1,2,1] = 0 
B[3,1,2,1,2,2] = 0 
B[3,1,2,2,1,1] = 0 
B[3,1,2,2,1,2] = 0 
B[3,1,2,2,2,1] = 0 
B[3,1,2,2,2,2] = 0 
B[3,1,3,1,1,1] = -1/(8*h[1]) 
B[3,1,3,1,1,2] = -1/(8*h[1]) 
B[3,1,3,1,2,1] = -1/(8*h[1]) 
B[3,1,3,1,2,2] = -1/(8*h[1]) 
B[3,1,3,2,1,1] = 1/(8*h[1]) 
B[3,1,3,2,1,2] = 1/(8*h[1]) 
B[3,1,3,2,2,1] = 1/(8*h[1]) 
B[3,1,3,2,2,2] = 1/(8*h[1]) 
B[3,2,1,1,1,1] = 0 
B[3,2,1,1,1,2] = 0 
B[3,2,1,1,2,1] = 0 
B[3,2,1,1,2,2] = 0 
B[3,2,1,2,1,1] = 0 
B[3,2,1,2,1,2] = 0 
B[3,2,1,2,2,1] = 0 
B[3,2,1,2,2,2] = 0 
B[3,2,2,1,1,1] = -1/(8*h[3]) 
B[3,2,2,1,1,2] = 1/(8*h[3]) 
B[3,2,2,1,2,1] = -1/(8*h[3]) 
B[3,2,2,1,2,2] = 1/(8*h[3]) 
B[3,2,2,2,1,1] = -1/(8*h[3]) 
B[3,2,2,2,1,2] = 1/(8*h[3]) 
B[3,2,2,2,2,1] = -1/(8*h[3]) 
B[3,2,2,2,2,2] = 1/(8*h[3]) 
B[3,2,3,1,1,1] = -1/(8*h[2]) 
B[3,2,3,1,1,2] = -1/(8*h[2]) 
B[3,2,3,1,2,1] = 1/(8*h[2]) 
B[3,2,3,1,2,2] = 1/(8*h[2]) 
B[3,2,3,2,1,1] = -1/(8*h[2]) 
B[3,2,3,2,1,2] = -1/(8*h[2]) 
B[3,2,3,2,2,1] = 1/(8*h[2]) 
B[3,2,3,2,2,2] = 1/(8*h[2]) 
B[3,3,1,1,1,1] = 0 
B[3,3,1,1,1,2] = 0 
B[3,3,1,1,2,1] = 0 
B[3,3,1,1,2,2] = 0 
B[3,3,1,2,1,1] = 0 
B[3,3,1,2,1,2] = 0 
B[3,3,1,2,2,1] = 0 
B[3,3,1,2,2,2] = 0 
B[3,3,2,1,1,1] = 0 
B[3,3,2,1,1,2] = 0 
B[3,3,2,1,2,1] = 0 
B[3,3,2,1,2,2] = 0 
B[3,3,2,2,1,1] = 0 
B[3,3,2,2,1,2] = 0 
B[3,3,2,2,2,1] = 0 
B[3,3,2,2,2,2] = 0 
B[3,3,3,1,1,1] = -1/(4*h[3]) 
B[3,3,3,1,1,2] = 1/(4*h[3]) 
B[3,3,3,1,2,1] = -1/(4*h[3]) 
B[3,3,3,1,2,2] = 1/(4*h[3]) 
B[3,3,3,2,1,1] = -1/(4*h[3]) 
B[3,3,3,2,1,2] = 1/(4*h[3]) 
B[3,3,3,2,2,1] = -1/(4*h[3]) 
B[3,3,3,2,2,2] = 1/(4*h[3]) 
``` 

## Stiffness matrix 

Testing that elastic energy is retrieved from extracted stiffness matrix... 
OK 

We get the following coefficients of the stiffness operator 
``` 

value = -h[1]/12 
K_λ[2,1,1,1,3,1,1,2] = value 
K_λ[2,1,1,1,3,1,2,2] = value 
K_λ[2,1,1,2,3,1,1,2] = value 
K_λ[2,1,1,2,3,1,2,2] = value 
K_λ[2,1,2,1,3,1,1,1] = value 
K_λ[2,1,2,1,3,1,2,1] = value 
K_λ[2,1,2,2,3,1,1,1] = value 
K_λ[2,1,2,2,3,1,2,1] = value 
K_λ[2,2,1,1,3,2,1,2] = value 
K_λ[2,2,1,1,3,2,2,2] = value 
K_λ[2,2,1,2,3,2,1,2] = value 
K_λ[2,2,1,2,3,2,2,2] = value 
K_λ[2,2,2,1,3,2,1,1] = value 
K_λ[2,2,2,1,3,2,2,1] = value 
K_λ[2,2,2,2,3,2,1,1] = value 
K_λ[2,2,2,2,3,2,2,1] = value 
K_λ[3,1,1,1,2,1,2,1] = value 
K_λ[3,1,1,1,2,1,2,2] = value 
K_λ[3,1,1,2,2,1,1,1] = value 
K_λ[3,1,1,2,2,1,1,2] = value 
K_λ[3,1,2,1,2,1,2,1] = value 
K_λ[3,1,2,1,2,1,2,2] = value 
K_λ[3,1,2,2,2,1,1,1] = value 
K_λ[3,1,2,2,2,1,1,2] = value 
K_λ[3,2,1,1,2,2,2,1] = value 
K_λ[3,2,1,1,2,2,2,2] = value 
K_λ[3,2,1,2,2,2,1,1] = value 
K_λ[3,2,1,2,2,2,1,2] = value 
K_λ[3,2,2,1,2,2,2,1] = value 
K_λ[3,2,2,1,2,2,2,2] = value 
K_λ[3,2,2,2,2,2,1,1] = value 
K_λ[3,2,2,2,2,2,1,2] = value 

value = -h[1]/24 
K_λ[2,1,1,1,3,2,1,2] = value 
K_λ[2,1,1,1,3,2,2,2] = value 
K_λ[2,1,1,2,3,2,1,2] = value 
K_λ[2,1,1,2,3,2,2,2] = value 
K_λ[2,1,2,1,3,2,1,1] = value 
K_λ[2,1,2,1,3,2,2,1] = value 
K_λ[2,1,2,2,3,2,1,1] = value 
K_λ[2,1,2,2,3,2,2,1] = value 
K_λ[2,2,1,1,3,1,1,2] = value 
K_λ[2,2,1,1,3,1,2,2] = value 
K_λ[2,2,1,2,3,1,1,2] = value 
K_λ[2,2,1,2,3,1,2,2] = value 
K_λ[2,2,2,1,3,1,1,1] = value 
K_λ[2,2,2,1,3,1,2,1] = value 
K_λ[2,2,2,2,3,1,1,1] = value 
K_λ[2,2,2,2,3,1,2,1] = value 
K_λ[3,1,1,1,2,2,2,1] = value 
K_λ[3,1,1,1,2,2,2,2] = value 
K_λ[3,1,1,2,2,2,1,1] = value 
K_λ[3,1,1,2,2,2,1,2] = value 
K_λ[3,1,2,1,2,2,2,1] = value 
K_λ[3,1,2,1,2,2,2,2] = value 
K_λ[3,1,2,2,2,2,1,1] = value 
K_λ[3,1,2,2,2,2,1,2] = value 
K_λ[3,2,1,1,2,1,2,1] = value 
K_λ[3,2,1,1,2,1,2,2] = value 
K_λ[3,2,1,2,2,1,1,1] = value 
K_λ[3,2,1,2,2,1,1,2] = value 
K_λ[3,2,2,1,2,1,2,1] = value 
K_λ[3,2,2,1,2,1,2,2] = value 
K_λ[3,2,2,2,2,1,1,1] = value 
K_λ[3,2,2,2,2,1,1,2] = value 

value = h[1]/24 
K_λ[2,1,1,1,3,2,1,1] = value 
K_λ[2,1,1,1,3,2,2,1] = value 
K_λ[2,1,1,2,3,2,1,1] = value 
K_λ[2,1,1,2,3,2,2,1] = value 
K_λ[2,1,2,1,3,2,1,2] = value 
K_λ[2,1,2,1,3,2,2,2] = value 
K_λ[2,1,2,2,3,2,1,2] = value 
K_λ[2,1,2,2,3,2,2,2] = value 
K_λ[2,2,1,1,3,1,1,1] = value 
K_λ[2,2,1,1,3,1,2,1] = value 
K_λ[2,2,1,2,3,1,1,1] = value 
K_λ[2,2,1,2,3,1,2,1] = value 
K_λ[2,2,2,1,3,1,1,2] = value 
K_λ[2,2,2,1,3,1,2,2] = value 
K_λ[2,2,2,2,3,1,1,2] = value 
K_λ[2,2,2,2,3,1,2,2] = value 
K_λ[3,1,1,1,2,2,1,1] = value 
K_λ[3,1,1,1,2,2,1,2] = value 
K_λ[3,1,1,2,2,2,2,1] = value 
K_λ[3,1,1,2,2,2,2,2] = value 
K_λ[3,1,2,1,2,2,1,1] = value 
K_λ[3,1,2,1,2,2,1,2] = value 
K_λ[3,1,2,2,2,2,2,1] = value 
K_λ[3,1,2,2,2,2,2,2] = value 
K_λ[3,2,1,1,2,1,1,1] = value 
K_λ[3,2,1,1,2,1,1,2] = value 
K_λ[3,2,1,2,2,1,2,1] = value 
K_λ[3,2,1,2,2,1,2,2] = value 
K_λ[3,2,2,1,2,1,1,1] = value 
K_λ[3,2,2,1,2,1,1,2] = value 
K_λ[3,2,2,2,2,1,2,1] = value 
K_λ[3,2,2,2,2,1,2,2] = value 

value = h[1]/12 
K_λ[2,1,1,1,3,1,1,1] = value 
K_λ[2,1,1,1,3,1,2,1] = value 
K_λ[2,1,1,2,3,1,1,1] = value 
K_λ[2,1,1,2,3,1,2,1] = value 
K_λ[2,1,2,1,3,1,1,2] = value 
K_λ[2,1,2,1,3,1,2,2] = value 
K_λ[2,1,2,2,3,1,1,2] = value 
K_λ[2,1,2,2,3,1,2,2] = value 
K_λ[2,2,1,1,3,2,1,1] = value 
K_λ[2,2,1,1,3,2,2,1] = value 
K_λ[2,2,1,2,3,2,1,1] = value 
K_λ[2,2,1,2,3,2,2,1] = value 
K_λ[2,2,2,1,3,2,1,2] = value 
K_λ[2,2,2,1,3,2,2,2] = value 
K_λ[2,2,2,2,3,2,1,2] = value 
K_λ[2,2,2,2,3,2,2,2] = value 
K_λ[3,1,1,1,2,1,1,1] = value 
K_λ[3,1,1,1,2,1,1,2] = value 
K_λ[3,1,1,2,2,1,2,1] = value 
K_λ[3,1,1,2,2,1,2,2] = value 
K_λ[3,1,2,1,2,1,1,1] = value 
K_λ[3,1,2,1,2,1,1,2] = value 
K_λ[3,1,2,2,2,1,2,1] = value 
K_λ[3,1,2,2,2,1,2,2] = value 
K_λ[3,2,1,1,2,2,1,1] = value 
K_λ[3,2,1,1,2,2,1,2] = value 
K_λ[3,2,1,2,2,2,2,1] = value 
K_λ[3,2,1,2,2,2,2,2] = value 
K_λ[3,2,2,1,2,2,1,1] = value 
K_λ[3,2,2,1,2,2,1,2] = value 
K_λ[3,2,2,2,2,2,2,1] = value 
K_λ[3,2,2,2,2,2,2,2] = value 

value = -h[2]/12 
K_λ[1,1,1,1,3,1,1,2] = value 
K_λ[1,1,1,1,3,2,1,2] = value 
K_λ[1,1,1,2,3,1,1,2] = value 
K_λ[1,1,1,2,3,2,1,2] = value 
K_λ[1,1,2,1,3,1,2,2] = value 
K_λ[1,1,2,1,3,2,2,2] = value 
K_λ[1,1,2,2,3,1,2,2] = value 
K_λ[1,1,2,2,3,2,2,2] = value 
K_λ[1,2,1,1,3,1,1,1] = value 
K_λ[1,2,1,1,3,2,1,1] = value 
K_λ[1,2,1,2,3,1,1,1] = value 
K_λ[1,2,1,2,3,2,1,1] = value 
K_λ[1,2,2,1,3,1,2,1] = value 
K_λ[1,2,2,1,3,2,2,1] = value 
K_λ[1,2,2,2,3,1,2,1] = value 
K_λ[1,2,2,2,3,2,2,1] = value 
K_λ[3,1,1,1,1,2,1,1] = value 
K_λ[3,1,1,1,1,2,1,2] = value 
K_λ[3,1,1,2,1,1,1,1] = value 
K_λ[3,1,1,2,1,1,1,2] = value 
K_λ[3,1,2,1,1,2,2,1] = value 
K_λ[3,1,2,1,1,2,2,2] = value 
K_λ[3,1,2,2,1,1,2,1] = value 
K_λ[3,1,2,2,1,1,2,2] = value 
K_λ[3,2,1,1,1,2,1,1] = value 
K_λ[3,2,1,1,1,2,1,2] = value 
K_λ[3,2,1,2,1,1,1,1] = value 
K_λ[3,2,1,2,1,1,1,2] = value 
K_λ[3,2,2,1,1,2,2,1] = value 
K_λ[3,2,2,1,1,2,2,2] = value 
K_λ[3,2,2,2,1,1,2,1] = value 
K_λ[3,2,2,2,1,1,2,2] = value 

value = -h[2]/24 
K_λ[1,1,1,1,3,1,2,2] = value 
K_λ[1,1,1,1,3,2,2,2] = value 
K_λ[1,1,1,2,3,1,2,2] = value 
K_λ[1,1,1,2,3,2,2,2] = value 
K_λ[1,1,2,1,3,1,1,2] = value 
K_λ[1,1,2,1,3,2,1,2] = value 
K_λ[1,1,2,2,3,1,1,2] = value 
K_λ[1,1,2,2,3,2,1,2] = value 
K_λ[1,2,1,1,3,1,2,1] = value 
K_λ[1,2,1,1,3,2,2,1] = value 
K_λ[1,2,1,2,3,1,2,1] = value 
K_λ[1,2,1,2,3,2,2,1] = value 
K_λ[1,2,2,1,3,1,1,1] = value 
K_λ[1,2,2,1,3,2,1,1] = value 
K_λ[1,2,2,2,3,1,1,1] = value 
K_λ[1,2,2,2,3,2,1,1] = value 
K_λ[3,1,1,1,1,2,2,1] = value 
K_λ[3,1,1,1,1,2,2,2] = value 
K_λ[3,1,1,2,1,1,2,1] = value 
K_λ[3,1,1,2,1,1,2,2] = value 
K_λ[3,1,2,1,1,2,1,1] = value 
K_λ[3,1,2,1,1,2,1,2] = value 
K_λ[3,1,2,2,1,1,1,1] = value 
K_λ[3,1,2,2,1,1,1,2] = value 
K_λ[3,2,1,1,1,2,2,1] = value 
K_λ[3,2,1,1,1,2,2,2] = value 
K_λ[3,2,1,2,1,1,2,1] = value 
K_λ[3,2,1,2,1,1,2,2] = value 
K_λ[3,2,2,1,1,2,1,1] = value 
K_λ[3,2,2,1,1,2,1,2] = value 
K_λ[3,2,2,2,1,1,1,1] = value 
K_λ[3,2,2,2,1,1,1,2] = value 

value = h[2]/24 
K_λ[1,1,1,1,3,1,2,1] = value 
K_λ[1,1,1,1,3,2,2,1] = value 
K_λ[1,1,1,2,3,1,2,1] = value 
K_λ[1,1,1,2,3,2,2,1] = value 
K_λ[1,1,2,1,3,1,1,1] = value 
K_λ[1,1,2,1,3,2,1,1] = value 
K_λ[1,1,2,2,3,1,1,1] = value 
K_λ[1,1,2,2,3,2,1,1] = value 
K_λ[1,2,1,1,3,1,2,2] = value 
K_λ[1,2,1,1,3,2,2,2] = value 
K_λ[1,2,1,2,3,1,2,2] = value 
K_λ[1,2,1,2,3,2,2,2] = value 
K_λ[1,2,2,1,3,1,1,2] = value 
K_λ[1,2,2,1,3,2,1,2] = value 
K_λ[1,2,2,2,3,1,1,2] = value 
K_λ[1,2,2,2,3,2,1,2] = value 
K_λ[3,1,1,1,1,1,2,1] = value 
K_λ[3,1,1,1,1,1,2,2] = value 
K_λ[3,1,1,2,1,2,2,1] = value 
K_λ[3,1,1,2,1,2,2,2] = value 
K_λ[3,1,2,1,1,1,1,1] = value 
K_λ[3,1,2,1,1,1,1,2] = value 
K_λ[3,1,2,2,1,2,1,1] = value 
K_λ[3,1,2,2,1,2,1,2] = value 
K_λ[3,2,1,1,1,1,2,1] = value 
K_λ[3,2,1,1,1,1,2,2] = value 
K_λ[3,2,1,2,1,2,2,1] = value 
K_λ[3,2,1,2,1,2,2,2] = value 
K_λ[3,2,2,1,1,1,1,1] = value 
K_λ[3,2,2,1,1,1,1,2] = value 
K_λ[3,2,2,2,1,2,1,1] = value 
K_λ[3,2,2,2,1,2,1,2] = value 

value = h[2]/12 
K_λ[1,1,1,1,3,1,1,1] = value 
K_λ[1,1,1,1,3,2,1,1] = value 
K_λ[1,1,1,2,3,1,1,1] = value 
K_λ[1,1,1,2,3,2,1,1] = value 
K_λ[1,1,2,1,3,1,2,1] = value 
K_λ[1,1,2,1,3,2,2,1] = value 
K_λ[1,1,2,2,3,1,2,1] = value 
K_λ[1,1,2,2,3,2,2,1] = value 
K_λ[1,2,1,1,3,1,1,2] = value 
K_λ[1,2,1,1,3,2,1,2] = value 
K_λ[1,2,1,2,3,1,1,2] = value 
K_λ[1,2,1,2,3,2,1,2] = value 
K_λ[1,2,2,1,3,1,2,2] = value 
K_λ[1,2,2,1,3,2,2,2] = value 
K_λ[1,2,2,2,3,1,2,2] = value 
K_λ[1,2,2,2,3,2,2,2] = value 
K_λ[3,1,1,1,1,1,1,1] = value 
K_λ[3,1,1,1,1,1,1,2] = value 
K_λ[3,1,1,2,1,2,1,1] = value 
K_λ[3,1,1,2,1,2,1,2] = value 
K_λ[3,1,2,1,1,1,2,1] = value 
K_λ[3,1,2,1,1,1,2,2] = value 
K_λ[3,1,2,2,1,2,2,1] = value 
K_λ[3,1,2,2,1,2,2,2] = value 
K_λ[3,2,1,1,1,1,1,1] = value 
K_λ[3,2,1,1,1,1,1,2] = value 
K_λ[3,2,1,2,1,2,1,1] = value 
K_λ[3,2,1,2,1,2,1,2] = value 
K_λ[3,2,2,1,1,1,2,1] = value 
K_λ[3,2,2,1,1,1,2,2] = value 
K_λ[3,2,2,2,1,2,2,1] = value 
K_λ[3,2,2,2,1,2,2,2] = value 

value = -(h[1]*h[2])/(9*h[3]) 
K_λ[3,1,1,1,3,1,1,2] = value 
K_λ[3,1,1,2,3,1,1,1] = value 
K_λ[3,1,2,1,3,1,2,2] = value 
K_λ[3,1,2,2,3,1,2,1] = value 
K_λ[3,2,1,1,3,2,1,2] = value 
K_λ[3,2,1,2,3,2,1,1] = value 
K_λ[3,2,2,1,3,2,2,2] = value 
K_λ[3,2,2,2,3,2,2,1] = value 

value = -(h[1]*h[2])/(18*h[3]) 
K_λ[3,1,1,1,3,1,2,2] = value 
K_λ[3,1,1,1,3,2,1,2] = value 
K_λ[3,1,1,2,3,1,2,1] = value 
K_λ[3,1,1,2,3,2,1,1] = value 
K_λ[3,1,2,1,3,1,1,2] = value 
K_λ[3,1,2,1,3,2,2,2] = value 
K_λ[3,1,2,2,3,1,1,1] = value 
K_λ[3,1,2,2,3,2,2,1] = value 
K_λ[3,2,1,1,3,1,1,2] = value 
K_λ[3,2,1,1,3,2,2,2] = value 
K_λ[3,2,1,2,3,1,1,1] = value 
K_λ[3,2,1,2,3,2,2,1] = value 
K_λ[3,2,2,1,3,1,2,2] = value 
K_λ[3,2,2,1,3,2,1,2] = value 
K_λ[3,2,2,2,3,1,2,1] = value 
K_λ[3,2,2,2,3,2,1,1] = value 

value = -(h[1]*h[2])/(36*h[3]) 
K_λ[3,1,1,1,3,2,2,2] = value 
K_λ[3,1,1,2,3,2,2,1] = value 
K_λ[3,1,2,1,3,2,1,2] = value 
K_λ[3,1,2,2,3,2,1,1] = value 
K_λ[3,2,1,1,3,1,2,2] = value 
K_λ[3,2,1,2,3,1,2,1] = value 
K_λ[3,2,2,1,3,1,1,2] = value 
K_λ[3,2,2,2,3,1,1,1] = value 

value = (h[1]*h[2])/(36*h[3]) 
K_λ[3,1,1,1,3,2,2,1] = value 
K_λ[3,1,1,2,3,2,2,2] = value 
K_λ[3,1,2,1,3,2,1,1] = value 
K_λ[3,1,2,2,3,2,1,2] = value 
K_λ[3,2,1,1,3,1,2,1] = value 
K_λ[3,2,1,2,3,1,2,2] = value 
K_λ[3,2,2,1,3,1,1,1] = value 
K_λ[3,2,2,2,3,1,1,2] = value 

value = (h[1]*h[2])/(18*h[3]) 
K_λ[3,1,1,1,3,1,2,1] = value 
K_λ[3,1,1,1,3,2,1,1] = value 
K_λ[3,1,1,2,3,1,2,2] = value 
K_λ[3,1,1,2,3,2,1,2] = value 
K_λ[3,1,2,1,3,1,1,1] = value 
K_λ[3,1,2,1,3,2,2,1] = value 
K_λ[3,1,2,2,3,1,1,2] = value 
K_λ[3,1,2,2,3,2,2,2] = value 
K_λ[3,2,1,1,3,1,1,1] = value 
K_λ[3,2,1,1,3,2,2,1] = value 
K_λ[3,2,1,2,3,1,1,2] = value 
K_λ[3,2,1,2,3,2,2,2] = value 
K_λ[3,2,2,1,3,1,2,1] = value 
K_λ[3,2,2,1,3,2,1,1] = value 
K_λ[3,2,2,2,3,1,2,2] = value 
K_λ[3,2,2,2,3,2,1,2] = value 

value = (h[1]*h[2])/(9*h[3]) 
K_λ[3,1,1,1,3,1,1,1] = value 
K_λ[3,1,1,2,3,1,1,2] = value 
K_λ[3,1,2,1,3,1,2,1] = value 
K_λ[3,1,2,2,3,1,2,2] = value 
K_λ[3,2,1,1,3,2,1,1] = value 
K_λ[3,2,1,2,3,2,1,2] = value 
K_λ[3,2,2,1,3,2,2,1] = value 
K_λ[3,2,2,2,3,2,2,2] = value 

value = -h[3]/12 
K_λ[1,1,1,1,2,1,2,1] = value 
K_λ[1,1,1,1,2,2,2,1] = value 
K_λ[1,1,1,2,2,1,2,2] = value 
K_λ[1,1,1,2,2,2,2,2] = value 
K_λ[1,1,2,1,2,1,2,1] = value 
K_λ[1,1,2,1,2,2,2,1] = value 
K_λ[1,1,2,2,2,1,2,2] = value 
K_λ[1,1,2,2,2,2,2,2] = value 
K_λ[1,2,1,1,2,1,1,1] = value 
K_λ[1,2,1,1,2,2,1,1] = value 
K_λ[1,2,1,2,2,1,1,2] = value 
K_λ[1,2,1,2,2,2,1,2] = value 
K_λ[1,2,2,1,2,1,1,1] = value 
K_λ[1,2,2,1,2,2,1,1] = value 
K_λ[1,2,2,2,2,1,1,2] = value 
K_λ[1,2,2,2,2,2,1,2] = value 
K_λ[2,1,1,1,1,2,1,1] = value 
K_λ[2,1,1,1,1,2,2,1] = value 
K_λ[2,1,1,2,1,2,1,2] = value 
K_λ[2,1,1,2,1,2,2,2] = value 
K_λ[2,1,2,1,1,1,1,1] = value 
K_λ[2,1,2,1,1,1,2,1] = value 
K_λ[2,1,2,2,1,1,1,2] = value 
K_λ[2,1,2,2,1,1,2,2] = value 
K_λ[2,2,1,1,1,2,1,1] = value 
K_λ[2,2,1,1,1,2,2,1] = value 
K_λ[2,2,1,2,1,2,1,2] = value 
K_λ[2,2,1,2,1,2,2,2] = value 
K_λ[2,2,2,1,1,1,1,1] = value 
K_λ[2,2,2,1,1,1,2,1] = value 
K_λ[2,2,2,2,1,1,1,2] = value 
K_λ[2,2,2,2,1,1,2,2] = value 

value = -h[3]/24 
K_λ[1,1,1,1,2,1,2,2] = value 
K_λ[1,1,1,1,2,2,2,2] = value 
K_λ[1,1,1,2,2,1,2,1] = value 
K_λ[1,1,1,2,2,2,2,1] = value 
K_λ[1,1,2,1,2,1,2,2] = value 
K_λ[1,1,2,1,2,2,2,2] = value 
K_λ[1,1,2,2,2,1,2,1] = value 
K_λ[1,1,2,2,2,2,2,1] = value 
K_λ[1,2,1,1,2,1,1,2] = value 
K_λ[1,2,1,1,2,2,1,2] = value 
K_λ[1,2,1,2,2,1,1,1] = value 
K_λ[1,2,1,2,2,2,1,1] = value 
K_λ[1,2,2,1,2,1,1,2] = value 
K_λ[1,2,2,1,2,2,1,2] = value 
K_λ[1,2,2,2,2,1,1,1] = value 
K_λ[1,2,2,2,2,2,1,1] = value 
K_λ[2,1,1,1,1,2,1,2] = value 
K_λ[2,1,1,1,1,2,2,2] = value 
K_λ[2,1,1,2,1,2,1,1] = value 
K_λ[2,1,1,2,1,2,2,1] = value 
K_λ[2,1,2,1,1,1,1,2] = value 
K_λ[2,1,2,1,1,1,2,2] = value 
K_λ[2,1,2,2,1,1,1,1] = value 
K_λ[2,1,2,2,1,1,2,1] = value 
K_λ[2,2,1,1,1,2,1,2] = value 
K_λ[2,2,1,1,1,2,2,2] = value 
K_λ[2,2,1,2,1,2,1,1] = value 
K_λ[2,2,1,2,1,2,2,1] = value 
K_λ[2,2,2,1,1,1,1,2] = value 
K_λ[2,2,2,1,1,1,2,2] = value 
K_λ[2,2,2,2,1,1,1,1] = value 
K_λ[2,2,2,2,1,1,2,1] = value 

value = h[3]/24 
K_λ[1,1,1,1,2,1,1,2] = value 
K_λ[1,1,1,1,2,2,1,2] = value 
K_λ[1,1,1,2,2,1,1,1] = value 
K_λ[1,1,1,2,2,2,1,1] = value 
K_λ[1,1,2,1,2,1,1,2] = value 
K_λ[1,1,2,1,2,2,1,2] = value 
K_λ[1,1,2,2,2,1,1,1] = value 
K_λ[1,1,2,2,2,2,1,1] = value 
K_λ[1,2,1,1,2,1,2,2] = value 
K_λ[1,2,1,1,2,2,2,2] = value 
K_λ[1,2,1,2,2,1,2,1] = value 
K_λ[1,2,1,2,2,2,2,1] = value 
K_λ[1,2,2,1,2,1,2,2] = value 
K_λ[1,2,2,1,2,2,2,2] = value 
K_λ[1,2,2,2,2,1,2,1] = value 
K_λ[1,2,2,2,2,2,2,1] = value 
K_λ[2,1,1,1,1,1,1,2] = value 
K_λ[2,1,1,1,1,1,2,2] = value 
K_λ[2,1,1,2,1,1,1,1] = value 
K_λ[2,1,1,2,1,1,2,1] = value 
K_λ[2,1,2,1,1,2,1,2] = value 
K_λ[2,1,2,1,1,2,2,2] = value 
K_λ[2,1,2,2,1,2,1,1] = value 
K_λ[2,1,2,2,1,2,2,1] = value 
K_λ[2,2,1,1,1,1,1,2] = value 
K_λ[2,2,1,1,1,1,2,2] = value 
K_λ[2,2,1,2,1,1,1,1] = value 
K_λ[2,2,1,2,1,1,2,1] = value 
K_λ[2,2,2,1,1,2,1,2] = value 
K_λ[2,2,2,1,1,2,2,2] = value 
K_λ[2,2,2,2,1,2,1,1] = value 
K_λ[2,2,2,2,1,2,2,1] = value 

value = h[3]/12 
K_λ[1,1,1,1,2,1,1,1] = value 
K_λ[1,1,1,1,2,2,1,1] = value 
K_λ[1,1,1,2,2,1,1,2] = value 
K_λ[1,1,1,2,2,2,1,2] = value 
K_λ[1,1,2,1,2,1,1,1] = value 
K_λ[1,1,2,1,2,2,1,1] = value 
K_λ[1,1,2,2,2,1,1,2] = value 
K_λ[1,1,2,2,2,2,1,2] = value 
K_λ[1,2,1,1,2,1,2,1] = value 
K_λ[1,2,1,1,2,2,2,1] = value 
K_λ[1,2,1,2,2,1,2,2] = value 
K_λ[1,2,1,2,2,2,2,2] = value 
K_λ[1,2,2,1,2,1,2,1] = value 
K_λ[1,2,2,1,2,2,2,1] = value 
K_λ[1,2,2,2,2,1,2,2] = value 
K_λ[1,2,2,2,2,2,2,2] = value 
K_λ[2,1,1,1,1,1,1,1] = value 
K_λ[2,1,1,1,1,1,2,1] = value 
K_λ[2,1,1,2,1,1,1,2] = value 
K_λ[2,1,1,2,1,1,2,2] = value 
K_λ[2,1,2,1,1,2,1,1] = value 
K_λ[2,1,2,1,1,2,2,1] = value 
K_λ[2,1,2,2,1,2,1,2] = value 
K_λ[2,1,2,2,1,2,2,2] = value 
K_λ[2,2,1,1,1,1,1,1] = value 
K_λ[2,2,1,1,1,1,2,1] = value 
K_λ[2,2,1,2,1,1,1,2] = value 
K_λ[2,2,1,2,1,1,2,2] = value 
K_λ[2,2,2,1,1,2,1,1] = value 
K_λ[2,2,2,1,1,2,2,1] = value 
K_λ[2,2,2,2,1,2,1,2] = value 
K_λ[2,2,2,2,1,2,2,2] = value 

value = -(h[1]*h[3])/(9*h[2]) 
K_λ[2,1,1,1,2,1,2,1] = value 
K_λ[2,1,1,2,2,1,2,2] = value 
K_λ[2,1,2,1,2,1,1,1] = value 
K_λ[2,1,2,2,2,1,1,2] = value 
K_λ[2,2,1,1,2,2,2,1] = value 
K_λ[2,2,1,2,2,2,2,2] = value 
K_λ[2,2,2,1,2,2,1,1] = value 
K_λ[2,2,2,2,2,2,1,2] = value 

value = -(h[1]*h[3])/(18*h[2]) 
K_λ[2,1,1,1,2,1,2,2] = value 
K_λ[2,1,1,1,2,2,2,1] = value 
K_λ[2,1,1,2,2,1,2,1] = value 
K_λ[2,1,1,2,2,2,2,2] = value 
K_λ[2,1,2,1,2,1,1,2] = value 
K_λ[2,1,2,1,2,2,1,1] = value 
K_λ[2,1,2,2,2,1,1,1] = value 
K_λ[2,1,2,2,2,2,1,2] = value 
K_λ[2,2,1,1,2,1,2,1] = value 
K_λ[2,2,1,1,2,2,2,2] = value 
K_λ[2,2,1,2,2,1,2,2] = value 
K_λ[2,2,1,2,2,2,2,1] = value 
K_λ[2,2,2,1,2,1,1,1] = value 
K_λ[2,2,2,1,2,2,1,2] = value 
K_λ[2,2,2,2,2,1,1,2] = value 
K_λ[2,2,2,2,2,2,1,1] = value 

value = -(h[1]*h[3])/(36*h[2]) 
K_λ[2,1,1,1,2,2,2,2] = value 
K_λ[2,1,1,2,2,2,2,1] = value 
K_λ[2,1,2,1,2,2,1,2] = value 
K_λ[2,1,2,2,2,2,1,1] = value 
K_λ[2,2,1,1,2,1,2,2] = value 
K_λ[2,2,1,2,2,1,2,1] = value 
K_λ[2,2,2,1,2,1,1,2] = value 
K_λ[2,2,2,2,2,1,1,1] = value 

value = (h[1]*h[3])/(36*h[2]) 
K_λ[2,1,1,1,2,2,1,2] = value 
K_λ[2,1,1,2,2,2,1,1] = value 
K_λ[2,1,2,1,2,2,2,2] = value 
K_λ[2,1,2,2,2,2,2,1] = value 
K_λ[2,2,1,1,2,1,1,2] = value 
K_λ[2,2,1,2,2,1,1,1] = value 
K_λ[2,2,2,1,2,1,2,2] = value 
K_λ[2,2,2,2,2,1,2,1] = value 

value = (h[1]*h[3])/(18*h[2]) 
K_λ[2,1,1,1,2,1,1,2] = value 
K_λ[2,1,1,1,2,2,1,1] = value 
K_λ[2,1,1,2,2,1,1,1] = value 
K_λ[2,1,1,2,2,2,1,2] = value 
K_λ[2,1,2,1,2,1,2,2] = value 
K_λ[2,1,2,1,2,2,2,1] = value 
K_λ[2,1,2,2,2,1,2,1] = value 
K_λ[2,1,2,2,2,2,2,2] = value 
K_λ[2,2,1,1,2,1,1,1] = value 
K_λ[2,2,1,1,2,2,1,2] = value 
K_λ[2,2,1,2,2,1,1,2] = value 
K_λ[2,2,1,2,2,2,1,1] = value 
K_λ[2,2,2,1,2,1,2,1] = value 
K_λ[2,2,2,1,2,2,2,2] = value 
K_λ[2,2,2,2,2,1,2,2] = value 
K_λ[2,2,2,2,2,2,2,1] = value 

value = (h[1]*h[3])/(9*h[2]) 
K_λ[2,1,1,1,2,1,1,1] = value 
K_λ[2,1,1,2,2,1,1,2] = value 
K_λ[2,1,2,1,2,1,2,1] = value 
K_λ[2,1,2,2,2,1,2,2] = value 
K_λ[2,2,1,1,2,2,1,1] = value 
K_λ[2,2,1,2,2,2,1,2] = value 
K_λ[2,2,2,1,2,2,2,1] = value 
K_λ[2,2,2,2,2,2,2,2] = value 

value = -(h[2]*h[3])/(9*h[1]) 
K_λ[1,1,1,1,1,2,1,1] = value 
K_λ[1,1,1,2,1,2,1,2] = value 
K_λ[1,1,2,1,1,2,2,1] = value 
K_λ[1,1,2,2,1,2,2,2] = value 
K_λ[1,2,1,1,1,1,1,1] = value 
K_λ[1,2,1,2,1,1,1,2] = value 
K_λ[1,2,2,1,1,1,2,1] = value 
K_λ[1,2,2,2,1,1,2,2] = value 

value = -(h[2]*h[3])/(18*h[1]) 
K_λ[1,1,1,1,1,2,1,2] = value 
K_λ[1,1,1,1,1,2,2,1] = value 
K_λ[1,1,1,2,1,2,1,1] = value 
K_λ[1,1,1,2,1,2,2,2] = value 
K_λ[1,1,2,1,1,2,1,1] = value 
K_λ[1,1,2,1,1,2,2,2] = value 
K_λ[1,1,2,2,1,2,1,2] = value 
K_λ[1,1,2,2,1,2,2,1] = value 
K_λ[1,2,1,1,1,1,1,2] = value 
K_λ[1,2,1,1,1,1,2,1] = value 
K_λ[1,2,1,2,1,1,1,1] = value 
K_λ[1,2,1,2,1,1,2,2] = value 
K_λ[1,2,2,1,1,1,1,1] = value 
K_λ[1,2,2,1,1,1,2,2] = value 
K_λ[1,2,2,2,1,1,1,2] = value 
K_λ[1,2,2,2,1,1,2,1] = value 

value = -(h[2]*h[3])/(36*h[1]) 
K_λ[1,1,1,1,1,2,2,2] = value 
K_λ[1,1,1,2,1,2,2,1] = value 
K_λ[1,1,2,1,1,2,1,2] = value 
K_λ[1,1,2,2,1,2,1,1] = value 
K_λ[1,2,1,1,1,1,2,2] = value 
K_λ[1,2,1,2,1,1,2,1] = value 
K_λ[1,2,2,1,1,1,1,2] = value 
K_λ[1,2,2,2,1,1,1,1] = value 

value = (h[2]*h[3])/(36*h[1]) 
K_λ[1,1,1,1,1,1,2,2] = value 
K_λ[1,1,1,2,1,1,2,1] = value 
K_λ[1,1,2,1,1,1,1,2] = value 
K_λ[1,1,2,2,1,1,1,1] = value 
K_λ[1,2,1,1,1,2,2,2] = value 
K_λ[1,2,1,2,1,2,2,1] = value 
K_λ[1,2,2,1,1,2,1,2] = value 
K_λ[1,2,2,2,1,2,1,1] = value 

value = (h[2]*h[3])/(18*h[1]) 
K_λ[1,1,1,1,1,1,1,2] = value 
K_λ[1,1,1,1,1,1,2,1] = value 
K_λ[1,1,1,2,1,1,1,1] = value 
K_λ[1,1,1,2,1,1,2,2] = value 
K_λ[1,1,2,1,1,1,1,1] = value 
K_λ[1,1,2,1,1,1,2,2] = value 
K_λ[1,1,2,2,1,1,1,2] = value 
K_λ[1,1,2,2,1,1,2,1] = value 
K_λ[1,2,1,1,1,2,1,2] = value 
K_λ[1,2,1,1,1,2,2,1] = value 
K_λ[1,2,1,2,1,2,1,1] = value 
K_λ[1,2,1,2,1,2,2,2] = value 
K_λ[1,2,2,1,1,2,1,1] = value 
K_λ[1,2,2,1,1,2,2,2] = value 
K_λ[1,2,2,2,1,2,1,2] = value 
K_λ[1,2,2,2,1,2,2,1] = value 

value = (h[2]*h[3])/(9*h[1]) 
K_λ[1,1,1,1,1,1,1,1] = value 
K_λ[1,1,1,2,1,1,1,2] = value 
K_λ[1,1,2,1,1,1,2,1] = value 
K_λ[1,1,2,2,1,1,2,2] = value 
K_λ[1,2,1,1,1,2,1,1] = value 
K_λ[1,2,1,2,1,2,1,2] = value 
K_λ[1,2,2,1,1,2,2,1] = value 
K_λ[1,2,2,2,1,2,2,2] = value 

value = -h[1]/12 
K_μ[2,1,1,1,3,1,2,1] = value 
K_μ[2,1,1,1,3,1,2,2] = value 
K_μ[2,1,1,2,3,1,1,1] = value 
K_μ[2,1,1,2,3,1,1,2] = value 
K_μ[2,1,2,1,3,1,2,1] = value 
K_μ[2,1,2,1,3,1,2,2] = value 
K_μ[2,1,2,2,3,1,1,1] = value 
K_μ[2,1,2,2,3,1,1,2] = value 
K_μ[2,2,1,1,3,2,2,1] = value 
K_μ[2,2,1,1,3,2,2,2] = value 
K_μ[2,2,1,2,3,2,1,1] = value 
K_μ[2,2,1,2,3,2,1,2] = value 
K_μ[2,2,2,1,3,2,2,1] = value 
K_μ[2,2,2,1,3,2,2,2] = value 
K_μ[2,2,2,2,3,2,1,1] = value 
K_μ[2,2,2,2,3,2,1,2] = value 
K_μ[3,1,1,1,2,1,1,2] = value 
K_μ[3,1,1,1,2,1,2,2] = value 
K_μ[3,1,1,2,2,1,1,2] = value 
K_μ[3,1,1,2,2,1,2,2] = value 
K_μ[3,1,2,1,2,1,1,1] = value 
K_μ[3,1,2,1,2,1,2,1] = value 
K_μ[3,1,2,2,2,1,1,1] = value 
K_μ[3,1,2,2,2,1,2,1] = value 
K_μ[3,2,1,1,2,2,1,2] = value 
K_μ[3,2,1,1,2,2,2,2] = value 
K_μ[3,2,1,2,2,2,1,2] = value 
K_μ[3,2,1,2,2,2,2,2] = value 
K_μ[3,2,2,1,2,2,1,1] = value 
K_μ[3,2,2,1,2,2,2,1] = value 
K_μ[3,2,2,2,2,2,1,1] = value 
K_μ[3,2,2,2,2,2,2,1] = value 

value = -h[1]/24 
K_μ[2,1,1,1,3,2,2,1] = value 
K_μ[2,1,1,1,3,2,2,2] = value 
K_μ[2,1,1,2,3,2,1,1] = value 
K_μ[2,1,1,2,3,2,1,2] = value 
K_μ[2,1,2,1,3,2,2,1] = value 
K_μ[2,1,2,1,3,2,2,2] = value 
K_μ[2,1,2,2,3,2,1,1] = value 
K_μ[2,1,2,2,3,2,1,2] = value 
K_μ[2,2,1,1,3,1,2,1] = value 
K_μ[2,2,1,1,3,1,2,2] = value 
K_μ[2,2,1,2,3,1,1,1] = value 
K_μ[2,2,1,2,3,1,1,2] = value 
K_μ[2,2,2,1,3,1,2,1] = value 
K_μ[2,2,2,1,3,1,2,2] = value 
K_μ[2,2,2,2,3,1,1,1] = value 
K_μ[2,2,2,2,3,1,1,2] = value 
K_μ[3,1,1,1,2,2,1,2] = value 
K_μ[3,1,1,1,2,2,2,2] = value 
K_μ[3,1,1,2,2,2,1,2] = value 
K_μ[3,1,1,2,2,2,2,2] = value 
K_μ[3,1,2,1,2,2,1,1] = value 
K_μ[3,1,2,1,2,2,2,1] = value 
K_μ[3,1,2,2,2,2,1,1] = value 
K_μ[3,1,2,2,2,2,2,1] = value 
K_μ[3,2,1,1,2,1,1,2] = value 
K_μ[3,2,1,1,2,1,2,2] = value 
K_μ[3,2,1,2,2,1,1,2] = value 
K_μ[3,2,1,2,2,1,2,2] = value 
K_μ[3,2,2,1,2,1,1,1] = value 
K_μ[3,2,2,1,2,1,2,1] = value 
K_μ[3,2,2,2,2,1,1,1] = value 
K_μ[3,2,2,2,2,1,2,1] = value 

value = h[1]/24 
K_μ[2,1,1,1,3,2,1,1] = value 
K_μ[2,1,1,1,3,2,1,2] = value 
K_μ[2,1,1,2,3,2,2,1] = value 
K_μ[2,1,1,2,3,2,2,2] = value 
K_μ[2,1,2,1,3,2,1,1] = value 
K_μ[2,1,2,1,3,2,1,2] = value 
K_μ[2,1,2,2,3,2,2,1] = value 
K_μ[2,1,2,2,3,2,2,2] = value 
K_μ[2,2,1,1,3,1,1,1] = value 
K_μ[2,2,1,1,3,1,1,2] = value 
K_μ[2,2,1,2,3,1,2,1] = value 
K_μ[2,2,1,2,3,1,2,2] = value 
K_μ[2,2,2,1,3,1,1,1] = value 
K_μ[2,2,2,1,3,1,1,2] = value 
K_μ[2,2,2,2,3,1,2,1] = value 
K_μ[2,2,2,2,3,1,2,2] = value 
K_μ[3,1,1,1,2,2,1,1] = value 
K_μ[3,1,1,1,2,2,2,1] = value 
K_μ[3,1,1,2,2,2,1,1] = value 
K_μ[3,1,1,2,2,2,2,1] = value 
K_μ[3,1,2,1,2,2,1,2] = value 
K_μ[3,1,2,1,2,2,2,2] = value 
K_μ[3,1,2,2,2,2,1,2] = value 
K_μ[3,1,2,2,2,2,2,2] = value 
K_μ[3,2,1,1,2,1,1,1] = value 
K_μ[3,2,1,1,2,1,2,1] = value 
K_μ[3,2,1,2,2,1,1,1] = value 
K_μ[3,2,1,2,2,1,2,1] = value 
K_μ[3,2,2,1,2,1,1,2] = value 
K_μ[3,2,2,1,2,1,2,2] = value 
K_μ[3,2,2,2,2,1,1,2] = value 
K_μ[3,2,2,2,2,1,2,2] = value 

value = h[1]/12 
K_μ[2,1,1,1,3,1,1,1] = value 
K_μ[2,1,1,1,3,1,1,2] = value 
K_μ[2,1,1,2,3,1,2,1] = value 
K_μ[2,1,1,2,3,1,2,2] = value 
K_μ[2,1,2,1,3,1,1,1] = value 
K_μ[2,1,2,1,3,1,1,2] = value 
K_μ[2,1,2,2,3,1,2,1] = value 
K_μ[2,1,2,2,3,1,2,2] = value 
K_μ[2,2,1,1,3,2,1,1] = value 
K_μ[2,2,1,1,3,2,1,2] = value 
K_μ[2,2,1,2,3,2,2,1] = value 
K_μ[2,2,1,2,3,2,2,2] = value 
K_μ[2,2,2,1,3,2,1,1] = value 
K_μ[2,2,2,1,3,2,1,2] = value 
K_μ[2,2,2,2,3,2,2,1] = value 
K_μ[2,2,2,2,3,2,2,2] = value 
K_μ[3,1,1,1,2,1,1,1] = value 
K_μ[3,1,1,1,2,1,2,1] = value 
K_μ[3,1,1,2,2,1,1,1] = value 
K_μ[3,1,1,2,2,1,2,1] = value 
K_μ[3,1,2,1,2,1,1,2] = value 
K_μ[3,1,2,1,2,1,2,2] = value 
K_μ[3,1,2,2,2,1,1,2] = value 
K_μ[3,1,2,2,2,1,2,2] = value 
K_μ[3,2,1,1,2,2,1,1] = value 
K_μ[3,2,1,1,2,2,2,1] = value 
K_μ[3,2,1,2,2,2,1,1] = value 
K_μ[3,2,1,2,2,2,2,1] = value 
K_μ[3,2,2,1,2,2,1,2] = value 
K_μ[3,2,2,1,2,2,2,2] = value 
K_μ[3,2,2,2,2,2,1,2] = value 
K_μ[3,2,2,2,2,2,2,2] = value 

value = -h[2]/12 
K_μ[1,1,1,1,3,2,1,1] = value 
K_μ[1,1,1,1,3,2,1,2] = value 
K_μ[1,1,1,2,3,1,1,1] = value 
K_μ[1,1,1,2,3,1,1,2] = value 
K_μ[1,1,2,1,3,2,2,1] = value 
K_μ[1,1,2,1,3,2,2,2] = value 
K_μ[1,1,2,2,3,1,2,1] = value 
K_μ[1,1,2,2,3,1,2,2] = value 
K_μ[1,2,1,1,3,2,1,1] = value 
K_μ[1,2,1,1,3,2,1,2] = value 
K_μ[1,2,1,2,3,1,1,1] = value 
K_μ[1,2,1,2,3,1,1,2] = value 
K_μ[1,2,2,1,3,2,2,1] = value 
K_μ[1,2,2,1,3,2,2,2] = value 
K_μ[1,2,2,2,3,1,2,1] = value 
K_μ[1,2,2,2,3,1,2,2] = value 
K_μ[3,1,1,1,1,1,1,2] = value 
K_μ[3,1,1,1,1,2,1,2] = value 
K_μ[3,1,1,2,1,1,1,2] = value 
K_μ[3,1,1,2,1,2,1,2] = value 
K_μ[3,1,2,1,1,1,2,2] = value 
K_μ[3,1,2,1,1,2,2,2] = value 
K_μ[3,1,2,2,1,1,2,2] = value 
K_μ[3,1,2,2,1,2,2,2] = value 
K_μ[3,2,1,1,1,1,1,1] = value 
K_μ[3,2,1,1,1,2,1,1] = value 
K_μ[3,2,1,2,1,1,1,1] = value 
K_μ[3,2,1,2,1,2,1,1] = value 
K_μ[3,2,2,1,1,1,2,1] = value 
K_μ[3,2,2,1,1,2,2,1] = value 
K_μ[3,2,2,2,1,1,2,1] = value 
K_μ[3,2,2,2,1,2,2,1] = value 

value = -h[2]/24 
K_μ[1,1,1,1,3,2,2,1] = value 
K_μ[1,1,1,1,3,2,2,2] = value 
K_μ[1,1,1,2,3,1,2,1] = value 
K_μ[1,1,1,2,3,1,2,2] = value 
K_μ[1,1,2,1,3,2,1,1] = value 
K_μ[1,1,2,1,3,2,1,2] = value 
K_μ[1,1,2,2,3,1,1,1] = value 
K_μ[1,1,2,2,3,1,1,2] = value 
K_μ[1,2,1,1,3,2,2,1] = value 
K_μ[1,2,1,1,3,2,2,2] = value 
K_μ[1,2,1,2,3,1,2,1] = value 
K_μ[1,2,1,2,3,1,2,2] = value 
K_μ[1,2,2,1,3,2,1,1] = value 
K_μ[1,2,2,1,3,2,1,2] = value 
K_μ[1,2,2,2,3,1,1,1] = value 
K_μ[1,2,2,2,3,1,1,2] = value 
K_μ[3,1,1,1,1,1,2,2] = value 
K_μ[3,1,1,1,1,2,2,2] = value 
K_μ[3,1,1,2,1,1,2,2] = value 
K_μ[3,1,1,2,1,2,2,2] = value 
K_μ[3,1,2,1,1,1,1,2] = value 
K_μ[3,1,2,1,1,2,1,2] = value 
K_μ[3,1,2,2,1,1,1,2] = value 
K_μ[3,1,2,2,1,2,1,2] = value 
K_μ[3,2,1,1,1,1,2,1] = value 
K_μ[3,2,1,1,1,2,2,1] = value 
K_μ[3,2,1,2,1,1,2,1] = value 
K_μ[3,2,1,2,1,2,2,1] = value 
K_μ[3,2,2,1,1,1,1,1] = value 
K_μ[3,2,2,1,1,2,1,1] = value 
K_μ[3,2,2,2,1,1,1,1] = value 
K_μ[3,2,2,2,1,2,1,1] = value 

value = h[2]/24 
K_μ[1,1,1,1,3,1,2,1] = value 
K_μ[1,1,1,1,3,1,2,2] = value 
K_μ[1,1,1,2,3,2,2,1] = value 
K_μ[1,1,1,2,3,2,2,2] = value 
K_μ[1,1,2,1,3,1,1,1] = value 
K_μ[1,1,2,1,3,1,1,2] = value 
K_μ[1,1,2,2,3,2,1,1] = value 
K_μ[1,1,2,2,3,2,1,2] = value 
K_μ[1,2,1,1,3,1,2,1] = value 
K_μ[1,2,1,1,3,1,2,2] = value 
K_μ[1,2,1,2,3,2,2,1] = value 
K_μ[1,2,1,2,3,2,2,2] = value 
K_μ[1,2,2,1,3,1,1,1] = value 
K_μ[1,2,2,1,3,1,1,2] = value 
K_μ[1,2,2,2,3,2,1,1] = value 
K_μ[1,2,2,2,3,2,1,2] = value 
K_μ[3,1,1,1,1,1,2,1] = value 
K_μ[3,1,1,1,1,2,2,1] = value 
K_μ[3,1,1,2,1,1,2,1] = value 
K_μ[3,1,1,2,1,2,2,1] = value 
K_μ[3,1,2,1,1,1,1,1] = value 
K_μ[3,1,2,1,1,2,1,1] = value 
K_μ[3,1,2,2,1,1,1,1] = value 
K_μ[3,1,2,2,1,2,1,1] = value 
K_μ[3,2,1,1,1,1,2,2] = value 
K_μ[3,2,1,1,1,2,2,2] = value 
K_μ[3,2,1,2,1,1,2,2] = value 
K_μ[3,2,1,2,1,2,2,2] = value 
K_μ[3,2,2,1,1,1,1,2] = value 
K_μ[3,2,2,1,1,2,1,2] = value 
K_μ[3,2,2,2,1,1,1,2] = value 
K_μ[3,2,2,2,1,2,1,2] = value 

value = h[2]/12 
K_μ[1,1,1,1,3,1,1,1] = value 
K_μ[1,1,1,1,3,1,1,2] = value 
K_μ[1,1,1,2,3,2,1,1] = value 
K_μ[1,1,1,2,3,2,1,2] = value 
K_μ[1,1,2,1,3,1,2,1] = value 
K_μ[1,1,2,1,3,1,2,2] = value 
K_μ[1,1,2,2,3,2,2,1] = value 
K_μ[1,1,2,2,3,2,2,2] = value 
K_μ[1,2,1,1,3,1,1,1] = value 
K_μ[1,2,1,1,3,1,1,2] = value 
K_μ[1,2,1,2,3,2,1,1] = value 
K_μ[1,2,1,2,3,2,1,2] = value 
K_μ[1,2,2,1,3,1,2,1] = value 
K_μ[1,2,2,1,3,1,2,2] = value 
K_μ[1,2,2,2,3,2,2,1] = value 
K_μ[1,2,2,2,3,2,2,2] = value 
K_μ[3,1,1,1,1,1,1,1] = value 
K_μ[3,1,1,1,1,2,1,1] = value 
K_μ[3,1,1,2,1,1,1,1] = value 
K_μ[3,1,1,2,1,2,1,1] = value 
K_μ[3,1,2,1,1,1,2,1] = value 
K_μ[3,1,2,1,1,2,2,1] = value 
K_μ[3,1,2,2,1,1,2,1] = value 
K_μ[3,1,2,2,1,2,2,1] = value 
K_μ[3,2,1,1,1,1,1,2] = value 
K_μ[3,2,1,1,1,2,1,2] = value 
K_μ[3,2,1,2,1,1,1,2] = value 
K_μ[3,2,1,2,1,2,1,2] = value 
K_μ[3,2,2,1,1,1,2,2] = value 
K_μ[3,2,2,1,1,2,2,2] = value 
K_μ[3,2,2,2,1,1,2,2] = value 
K_μ[3,2,2,2,1,2,2,2] = value 

value = -h[3]/12 
K_μ[1,1,1,1,2,2,1,1] = value 
K_μ[1,1,1,1,2,2,2,1] = value 
K_μ[1,1,1,2,2,2,1,2] = value 
K_μ[1,1,1,2,2,2,2,2] = value 
K_μ[1,1,2,1,2,1,1,1] = value 
K_μ[1,1,2,1,2,1,2,1] = value 
K_μ[1,1,2,2,2,1,1,2] = value 
K_μ[1,1,2,2,2,1,2,2] = value 
K_μ[1,2,1,1,2,2,1,1] = value 
K_μ[1,2,1,1,2,2,2,1] = value 
K_μ[1,2,1,2,2,2,1,2] = value 
K_μ[1,2,1,2,2,2,2,2] = value 
K_μ[1,2,2,1,2,1,1,1] = value 
K_μ[1,2,2,1,2,1,2,1] = value 
K_μ[1,2,2,2,2,1,1,2] = value 
K_μ[1,2,2,2,2,1,2,2] = value 
K_μ[2,1,1,1,1,1,2,1] = value 
K_μ[2,1,1,1,1,2,2,1] = value 
K_μ[2,1,1,2,1,1,2,2] = value 
K_μ[2,1,1,2,1,2,2,2] = value 
K_μ[2,1,2,1,1,1,2,1] = value 
K_μ[2,1,2,1,1,2,2,1] = value 
K_μ[2,1,2,2,1,1,2,2] = value 
K_μ[2,1,2,2,1,2,2,2] = value 
K_μ[2,2,1,1,1,1,1,1] = value 
K_μ[2,2,1,1,1,2,1,1] = value 
K_μ[2,2,1,2,1,1,1,2] = value 
K_μ[2,2,1,2,1,2,1,2] = value 
K_μ[2,2,2,1,1,1,1,1] = value 
K_μ[2,2,2,1,1,2,1,1] = value 
K_μ[2,2,2,2,1,1,1,2] = value 
K_μ[2,2,2,2,1,2,1,2] = value 

value = -h[3]/24 
K_μ[1,1,1,1,2,2,1,2] = value 
K_μ[1,1,1,1,2,2,2,2] = value 
K_μ[1,1,1,2,2,2,1,1] = value 
K_μ[1,1,1,2,2,2,2,1] = value 
K_μ[1,1,2,1,2,1,1,2] = value 
K_μ[1,1,2,1,2,1,2,2] = value 
K_μ[1,1,2,2,2,1,1,1] = value 
K_μ[1,1,2,2,2,1,2,1] = value 
K_μ[1,2,1,1,2,2,1,2] = value 
K_μ[1,2,1,1,2,2,2,2] = value 
K_μ[1,2,1,2,2,2,1,1] = value 
K_μ[1,2,1,2,2,2,2,1] = value 
K_μ[1,2,2,1,2,1,1,2] = value 
K_μ[1,2,2,1,2,1,2,2] = value 
K_μ[1,2,2,2,2,1,1,1] = value 
K_μ[1,2,2,2,2,1,2,1] = value 
K_μ[2,1,1,1,1,1,2,2] = value 
K_μ[2,1,1,1,1,2,2,2] = value 
K_μ[2,1,1,2,1,1,2,1] = value 
K_μ[2,1,1,2,1,2,2,1] = value 
K_μ[2,1,2,1,1,1,2,2] = value 
K_μ[2,1,2,1,1,2,2,2] = value 
K_μ[2,1,2,2,1,1,2,1] = value 
K_μ[2,1,2,2,1,2,2,1] = value 
K_μ[2,2,1,1,1,1,1,2] = value 
K_μ[2,2,1,1,1,2,1,2] = value 
K_μ[2,2,1,2,1,1,1,1] = value 
K_μ[2,2,1,2,1,2,1,1] = value 
K_μ[2,2,2,1,1,1,1,2] = value 
K_μ[2,2,2,1,1,2,1,2] = value 
K_μ[2,2,2,2,1,1,1,1] = value 
K_μ[2,2,2,2,1,2,1,1] = value 

value = h[3]/24 
K_μ[1,1,1,1,2,1,1,2] = value 
K_μ[1,1,1,1,2,1,2,2] = value 
K_μ[1,1,1,2,2,1,1,1] = value 
K_μ[1,1,1,2,2,1,2,1] = value 
K_μ[1,1,2,1,2,2,1,2] = value 
K_μ[1,1,2,1,2,2,2,2] = value 
K_μ[1,1,2,2,2,2,1,1] = value 
K_μ[1,1,2,2,2,2,2,1] = value 
K_μ[1,2,1,1,2,1,1,2] = value 
K_μ[1,2,1,1,2,1,2,2] = value 
K_μ[1,2,1,2,2,1,1,1] = value 
K_μ[1,2,1,2,2,1,2,1] = value 
K_μ[1,2,2,1,2,2,1,2] = value 
K_μ[1,2,2,1,2,2,2,2] = value 
K_μ[1,2,2,2,2,2,1,1] = value 
K_μ[1,2,2,2,2,2,2,1] = value 
K_μ[2,1,1,1,1,1,1,2] = value 
K_μ[2,1,1,1,1,2,1,2] = value 
K_μ[2,1,1,2,1,1,1,1] = value 
K_μ[2,1,1,2,1,2,1,1] = value 
K_μ[2,1,2,1,1,1,1,2] = value 
K_μ[2,1,2,1,1,2,1,2] = value 
K_μ[2,1,2,2,1,1,1,1] = value 
K_μ[2,1,2,2,1,2,1,1] = value 
K_μ[2,2,1,1,1,1,2,2] = value 
K_μ[2,2,1,1,1,2,2,2] = value 
K_μ[2,2,1,2,1,1,2,1] = value 
K_μ[2,2,1,2,1,2,2,1] = value 
K_μ[2,2,2,1,1,1,2,2] = value 
K_μ[2,2,2,1,1,2,2,2] = value 
K_μ[2,2,2,2,1,1,2,1] = value 
K_μ[2,2,2,2,1,2,2,1] = value 

value = h[3]/12 
K_μ[1,1,1,1,2,1,1,1] = value 
K_μ[1,1,1,1,2,1,2,1] = value 
K_μ[1,1,1,2,2,1,1,2] = value 
K_μ[1,1,1,2,2,1,2,2] = value 
K_μ[1,1,2,1,2,2,1,1] = value 
K_μ[1,1,2,1,2,2,2,1] = value 
K_μ[1,1,2,2,2,2,1,2] = value 
K_μ[1,1,2,2,2,2,2,2] = value 
K_μ[1,2,1,1,2,1,1,1] = value 
K_μ[1,2,1,1,2,1,2,1] = value 
K_μ[1,2,1,2,2,1,1,2] = value 
K_μ[1,2,1,2,2,1,2,2] = value 
K_μ[1,2,2,1,2,2,1,1] = value 
K_μ[1,2,2,1,2,2,2,1] = value 
K_μ[1,2,2,2,2,2,1,2] = value 
K_μ[1,2,2,2,2,2,2,2] = value 
K_μ[2,1,1,1,1,1,1,1] = value 
K_μ[2,1,1,1,1,2,1,1] = value 
K_μ[2,1,1,2,1,1,1,2] = value 
K_μ[2,1,1,2,1,2,1,2] = value 
K_μ[2,1,2,1,1,1,1,1] = value 
K_μ[2,1,2,1,1,2,1,1] = value 
K_μ[2,1,2,2,1,1,1,2] = value 
K_μ[2,1,2,2,1,2,1,2] = value 
K_μ[2,2,1,1,1,1,2,1] = value 
K_μ[2,2,1,1,1,2,2,1] = value 
K_μ[2,2,1,2,1,1,2,2] = value 
K_μ[2,2,1,2,1,2,2,2] = value 
K_μ[2,2,2,1,1,1,2,1] = value 
K_μ[2,2,2,1,1,2,2,1] = value 
K_μ[2,2,2,2,1,1,2,2] = value 
K_μ[2,2,2,2,1,2,2,2] = value 

value = (-(2*h[2]*h[3])/(9*h[1]))+(h[1]*h[3])/(18*h[2])+(h[1]*h[2])/(18*h[3]) 
K_μ[1,1,1,1,1,2,1,1] = value 
K_μ[1,1,1,2,1,2,1,2] = value 
K_μ[1,1,2,1,1,2,2,1] = value 
K_μ[1,1,2,2,1,2,2,2] = value 
K_μ[1,2,1,1,1,1,1,1] = value 
K_μ[1,2,1,2,1,1,1,2] = value 
K_μ[1,2,2,1,1,1,2,1] = value 
K_μ[1,2,2,2,1,1,2,2] = value 

value = (-(h[2]*h[3])/(9*h[1]))-(h[1]*h[3])/(18*h[2])+(h[1]*h[2])/(36*h[3]) 
K_μ[1,1,1,1,1,2,2,1] = value 
K_μ[1,1,1,2,1,2,2,2] = value 
K_μ[1,1,2,1,1,2,1,1] = value 
K_μ[1,1,2,2,1,2,1,2] = value 
K_μ[1,2,1,1,1,1,2,1] = value 
K_μ[1,2,1,2,1,1,2,2] = value 
K_μ[1,2,2,1,1,1,1,1] = value 
K_μ[1,2,2,2,1,1,1,2] = value 

value = (-(h[2]*h[3])/(9*h[1]))+(h[1]*h[3])/(36*h[2])-(h[1]*h[2])/(18*h[3]) 
K_μ[1,1,1,1,1,2,1,2] = value 
K_μ[1,1,1,2,1,2,1,1] = value 
K_μ[1,1,2,1,1,2,2,2] = value 
K_μ[1,1,2,2,1,2,2,1] = value 
K_μ[1,2,1,1,1,1,1,2] = value 
K_μ[1,2,1,2,1,1,1,1] = value 
K_μ[1,2,2,1,1,1,2,2] = value 
K_μ[1,2,2,2,1,1,2,1] = value 

value = (-(h[2]*h[3])/(9*h[1]))+(h[1]*h[3])/(18*h[2])+(h[1]*h[2])/(9*h[3]) 
K_μ[3,1,1,1,3,2,1,1] = value 
K_μ[3,1,1,2,3,2,1,2] = value 
K_μ[3,1,2,1,3,2,2,1] = value 
K_μ[3,1,2,2,3,2,2,2] = value 
K_μ[3,2,1,1,3,1,1,1] = value 
K_μ[3,2,1,2,3,1,1,2] = value 
K_μ[3,2,2,1,3,1,2,1] = value 
K_μ[3,2,2,2,3,1,2,2] = value 

value = (-(h[2]*h[3])/(9*h[1]))+(h[1]*h[3])/(9*h[2])+(h[1]*h[2])/(18*h[3]) 
K_μ[2,1,1,1,2,2,1,1] = value 
K_μ[2,1,1,2,2,2,1,2] = value 
K_μ[2,1,2,1,2,2,2,1] = value 
K_μ[2,1,2,2,2,2,2,2] = value 
K_μ[2,2,1,1,2,1,1,1] = value 
K_μ[2,2,1,2,2,1,1,2] = value 
K_μ[2,2,2,1,2,1,2,1] = value 
K_μ[2,2,2,2,2,1,2,2] = value 

value = (-(h[2]*h[3])/(18*h[1]))-(h[1]*h[3])/(9*h[2])+(h[1]*h[2])/(36*h[3]) 
K_μ[2,1,1,1,2,2,2,1] = value 
K_μ[2,1,1,2,2,2,2,2] = value 
K_μ[2,1,2,1,2,2,1,1] = value 
K_μ[2,1,2,2,2,2,1,2] = value 
K_μ[2,2,1,1,2,1,2,1] = value 
K_μ[2,2,1,2,2,1,2,2] = value 
K_μ[2,2,2,1,2,1,1,1] = value 
K_μ[2,2,2,2,2,1,1,2] = value 

value = (-(h[2]*h[3])/(18*h[1]))-(h[1]*h[3])/(18*h[2])+(h[1]*h[2])/(18*h[3]) 
K_μ[3,1,1,1,3,2,2,1] = value 
K_μ[3,1,1,2,3,2,2,2] = value 
K_μ[3,1,2,1,3,2,1,1] = value 
K_μ[3,1,2,2,3,2,1,2] = value 
K_μ[3,2,1,1,3,1,2,1] = value 
K_μ[3,2,1,2,3,1,2,2] = value 
K_μ[3,2,2,1,3,1,1,1] = value 
K_μ[3,2,2,2,3,1,1,2] = value 

value = (-(h[2]*h[3])/(18*h[1]))-(h[1]*h[3])/(36*h[2])-(h[1]*h[2])/(36*h[3]) 
K_μ[1,1,1,1,1,2,2,2] = value 
K_μ[1,1,1,2,1,2,2,1] = value 
K_μ[1,1,2,1,1,2,1,2] = value 
K_μ[1,1,2,2,1,2,1,1] = value 
K_μ[1,2,1,1,1,1,2,2] = value 
K_μ[1,2,1,2,1,1,2,1] = value 
K_μ[1,2,2,1,1,1,1,2] = value 
K_μ[1,2,2,2,1,1,1,1] = value 

value = (-(h[2]*h[3])/(18*h[1]))+(h[1]*h[3])/(36*h[2])-(h[1]*h[2])/(9*h[3]) 
K_μ[3,1,1,1,3,2,1,2] = value 
K_μ[3,1,1,2,3,2,1,1] = value 
K_μ[3,1,2,1,3,2,2,2] = value 
K_μ[3,1,2,2,3,2,2,1] = value 
K_μ[3,2,1,1,3,1,1,2] = value 
K_μ[3,2,1,2,3,1,1,1] = value 
K_μ[3,2,2,1,3,1,2,2] = value 
K_μ[3,2,2,2,3,1,2,1] = value 

value = (-(h[2]*h[3])/(18*h[1]))+(h[1]*h[3])/(18*h[2])-(h[1]*h[2])/(18*h[3]) 
K_μ[2,1,1,1,2,2,1,2] = value 
K_μ[2,1,1,2,2,2,1,1] = value 
K_μ[2,1,2,1,2,2,2,2] = value 
K_μ[2,1,2,2,2,2,2,1] = value 
K_μ[2,2,1,1,2,1,1,2] = value 
K_μ[2,2,1,2,2,1,1,1] = value 
K_μ[2,2,2,1,2,1,2,2] = value 
K_μ[2,2,2,2,2,1,2,1] = value 

value = (-(h[2]*h[3])/(36*h[1]))-(h[1]*h[3])/(18*h[2])-(h[1]*h[2])/(36*h[3]) 
K_μ[2,1,1,1,2,2,2,2] = value 
K_μ[2,1,1,2,2,2,2,1] = value 
K_μ[2,1,2,1,2,2,1,2] = value 
K_μ[2,1,2,2,2,2,1,1] = value 
K_μ[2,2,1,1,2,1,2,2] = value 
K_μ[2,2,1,2,2,1,2,1] = value 
K_μ[2,2,2,1,2,1,1,2] = value 
K_μ[2,2,2,2,2,1,1,1] = value 

value = (-(h[2]*h[3])/(36*h[1]))-(h[1]*h[3])/(36*h[2])-(h[1]*h[2])/(18*h[3]) 
K_μ[3,1,1,1,3,2,2,2] = value 
K_μ[3,1,1,2,3,2,2,1] = value 
K_μ[3,1,2,1,3,2,1,2] = value 
K_μ[3,1,2,2,3,2,1,1] = value 
K_μ[3,2,1,1,3,1,2,2] = value 
K_μ[3,2,1,2,3,1,2,1] = value 
K_μ[3,2,2,1,3,1,1,2] = value 
K_μ[3,2,2,2,3,1,1,1] = value 

value = (h[2]*h[3])/(36*h[1])-(h[1]*h[3])/(9*h[2])-(h[1]*h[2])/(18*h[3]) 
K_μ[2,1,1,1,2,1,2,2] = value 
K_μ[2,1,1,2,2,1,2,1] = value 
K_μ[2,1,2,1,2,1,1,2] = value 
K_μ[2,1,2,2,2,1,1,1] = value 
K_μ[2,2,1,1,2,2,2,2] = value 
K_μ[2,2,1,2,2,2,2,1] = value 
K_μ[2,2,2,1,2,2,1,2] = value 
K_μ[2,2,2,2,2,2,1,1] = value 

value = (h[2]*h[3])/(36*h[1])-(h[1]*h[3])/(18*h[2])-(h[1]*h[2])/(9*h[3]) 
K_μ[3,1,1,1,3,1,2,2] = value 
K_μ[3,1,1,2,3,1,2,1] = value 
K_μ[3,1,2,1,3,1,1,2] = value 
K_μ[3,1,2,2,3,1,1,1] = value 
K_μ[3,2,1,1,3,2,2,2] = value 
K_μ[3,2,1,2,3,2,2,1] = value 
K_μ[3,2,2,1,3,2,1,2] = value 
K_μ[3,2,2,2,3,2,1,1] = value 

value = (h[2]*h[3])/(18*h[1])-(2*h[1]*h[3])/(9*h[2])+(h[1]*h[2])/(18*h[3]) 
K_μ[2,1,1,1,2,1,2,1] = value 
K_μ[2,1,1,2,2,1,2,2] = value 
K_μ[2,1,2,1,2,1,1,1] = value 
K_μ[2,1,2,2,2,1,1,2] = value 
K_μ[2,2,1,1,2,2,2,1] = value 
K_μ[2,2,1,2,2,2,2,2] = value 
K_μ[2,2,2,1,2,2,1,1] = value 
K_μ[2,2,2,2,2,2,1,2] = value 

value = (h[2]*h[3])/(18*h[1])-(h[1]*h[3])/(9*h[2])+(h[1]*h[2])/(9*h[3]) 
K_μ[3,1,1,1,3,1,2,1] = value 
K_μ[3,1,1,2,3,1,2,2] = value 
K_μ[3,1,2,1,3,1,1,1] = value 
K_μ[3,1,2,2,3,1,1,2] = value 
K_μ[3,2,1,1,3,2,2,1] = value 
K_μ[3,2,1,2,3,2,2,2] = value 
K_μ[3,2,2,1,3,2,1,1] = value 
K_μ[3,2,2,2,3,2,1,2] = value 

value = (h[2]*h[3])/(18*h[1])-(h[1]*h[3])/(18*h[2])-(h[1]*h[2])/(18*h[3]) 
K_μ[1,1,1,1,1,1,2,2] = value 
K_μ[1,1,1,2,1,1,2,1] = value 
K_μ[1,1,2,1,1,1,1,2] = value 
K_μ[1,1,2,2,1,1,1,1] = value 
K_μ[1,2,1,1,1,2,2,2] = value 
K_μ[1,2,1,2,1,2,2,1] = value 
K_μ[1,2,2,1,1,2,1,2] = value 
K_μ[1,2,2,2,1,2,1,1] = value 

value = (h[2]*h[3])/(18*h[1])+(h[1]*h[3])/(18*h[2])-(2*h[1]*h[2])/(9*h[3]) 
K_μ[3,1,1,1,3,1,1,2] = value 
K_μ[3,1,1,2,3,1,1,1] = value 
K_μ[3,1,2,1,3,1,2,2] = value 
K_μ[3,1,2,2,3,1,2,1] = value 
K_μ[3,2,1,1,3,2,1,2] = value 
K_μ[3,2,1,2,3,2,1,1] = value 
K_μ[3,2,2,1,3,2,2,2] = value 
K_μ[3,2,2,2,3,2,2,1] = value 

value = (h[2]*h[3])/(18*h[1])+(h[1]*h[3])/(9*h[2])-(h[1]*h[2])/(9*h[3]) 
K_μ[2,1,1,1,2,1,1,2] = value 
K_μ[2,1,1,2,2,1,1,1] = value 
K_μ[2,1,2,1,2,1,2,2] = value 
K_μ[2,1,2,2,2,1,2,1] = value 
K_μ[2,2,1,1,2,2,1,2] = value 
K_μ[2,2,1,2,2,2,1,1] = value 
K_μ[2,2,2,1,2,2,2,2] = value 
K_μ[2,2,2,2,2,2,2,1] = value 

value = (h[2]*h[3])/(9*h[1])-(h[1]*h[3])/(9*h[2])+(h[1]*h[2])/(18*h[3]) 
K_μ[1,1,1,1,1,1,2,1] = value 
K_μ[1,1,1,2,1,1,2,2] = value 
K_μ[1,1,2,1,1,1,1,1] = value 
K_μ[1,1,2,2,1,1,1,2] = value 
K_μ[1,2,1,1,1,2,2,1] = value 
K_μ[1,2,1,2,1,2,2,2] = value 
K_μ[1,2,2,1,1,2,1,1] = value 
K_μ[1,2,2,2,1,2,1,2] = value 

value = (h[2]*h[3])/(9*h[1])+(h[1]*h[3])/(18*h[2])-(h[1]*h[2])/(9*h[3]) 
K_μ[1,1,1,1,1,1,1,2] = value 
K_μ[1,1,1,2,1,1,1,1] = value 
K_μ[1,1,2,1,1,1,2,2] = value 
K_μ[1,1,2,2,1,1,2,1] = value 
K_μ[1,2,1,1,1,2,1,2] = value 
K_μ[1,2,1,2,1,2,1,1] = value 
K_μ[1,2,2,1,1,2,2,2] = value 
K_μ[1,2,2,2,1,2,2,1] = value 

value = (h[2]*h[3])/(9*h[1])+(h[1]*h[3])/(9*h[2])+(2*h[1]*h[2])/(9*h[3]) 
K_μ[3,1,1,1,3,1,1,1] = value 
K_μ[3,1,1,2,3,1,1,2] = value 
K_μ[3,1,2,1,3,1,2,1] = value 
K_μ[3,1,2,2,3,1,2,2] = value 
K_μ[3,2,1,1,3,2,1,1] = value 
K_μ[3,2,1,2,3,2,1,2] = value 
K_μ[3,2,2,1,3,2,2,1] = value 
K_μ[3,2,2,2,3,2,2,2] = value 

value = (h[2]*h[3])/(9*h[1])+(2*h[1]*h[3])/(9*h[2])+(h[1]*h[2])/(9*h[3]) 
K_μ[2,1,1,1,2,1,1,1] = value 
K_μ[2,1,1,2,2,1,1,2] = value 
K_μ[2,1,2,1,2,1,2,1] = value 
K_μ[2,1,2,2,2,1,2,2] = value 
K_μ[2,2,1,1,2,2,1,1] = value 
K_μ[2,2,1,2,2,2,1,2] = value 
K_μ[2,2,2,1,2,2,2,1] = value 
K_μ[2,2,2,2,2,2,2,2] = value 

value = (2*h[2]*h[3])/(9*h[1])+(h[1]*h[3])/(9*h[2])+(h[1]*h[2])/(9*h[3]) 
K_μ[1,1,1,1,1,1,1,1] = value 
K_μ[1,1,1,2,1,1,1,2] = value 
K_μ[1,1,2,1,1,1,2,1] = value 
K_μ[1,1,2,2,1,1,2,2] = value 
K_μ[1,2,1,1,1,2,1,1] = value 
K_μ[1,2,1,2,1,2,1,2] = value 
K_μ[1,2,2,1,1,2,2,1] = value 
K_μ[1,2,2,2,1,2,2,2] = value 
``` 
